started working on machine that checks inout for Multi2Mono

theories/L/Complexity/Reductions/TMGenNP/mTM_to_singleTapeTM.v
@@ -1,18 +1,189 @@
+(* -*- coq-prefer-top-of-conclusion: t; -*- *)
 From Undecidability.L Require Import Tactics.LTactics.
 From Undecidability.L.Datatypes Require Import Lists LVector.
 From Undecidability.L.Complexity Require Import NP Synthetic Monotonic.
-From Undecidability.TM Require Import TM Single.StepTM.
+From Undecidability.TM Require Import TM ProgrammingTools.
 
 From Undecidability.L.Complexity  Require GenNP.
 From Undecidability.L.Complexity  Require Import LMGenNP TMGenNP_fixed_mTM.
 
 
-From Undecidability Require Import TM.Single.EncodeTapes.
+From Undecidability.TM Require Single.EncodeTapes Single.StepTM CaseList.
 
+
+
+
+Module ContainsEncoding.
+  Section containsEncoding.
+    Local Unset Implicit Arguments.
+    
+    Context {sig:Type} {n:nat} {X:Type}.
+    Context (d:sig) (encode : X -> list sig).
+    (*Hypothesis (nonEmpty : forall x, encode x <> []).*)
+
+    Definition Rel : pRel sig bool 1 :=
+      fun tin '(yout, tout) =>
+        inhabited
+          (reflect
+             (exists t__L (x:X) t__R,
+                 let t__x := encode x in
+                 tin[@Fin0] = midtape t__L (hd d t__x) (tl t__x++t__R)
+                 /\ tout[@Fin0] = midtape (rev (removelast t__x)++ t__L) (last t__x d) t__R)
+             yout).
+    
+  End containsEncoding.
+End ContainsEncoding.
+
+From Coq.ssr Require Import ssrfun.
+Module CheckEncodesTape.
+  Section checkEncodesTape.
+    
+    Import EncodeTapes StateWhile CaseList Mono Multi MoveToSymbol Switch If Combinators Option.
+    Context (sig:finType) (n:nat).
+
+    Compute encode_tape (midtape [3;2;1] 4 [5;6;7]).
+  (*encode_tape = 
+    fun (sig : Type) (t : tape sig) =>
+      match t with
+      | niltape _ => [NilBlank]
+      | leftof r rs => LeftBlank true :: UnmarkedSymbol r :: map UnmarkedSymbol rs ++ [RightBlank false]
+      | rightof l ls => LeftBlank false :: map UnmarkedSymbol (rev ls) ++ [UnmarkedSymbol l; RightBlank true]
+      | midtape ls m rs => LeftBlank false :: map UnmarkedSymbol (rev ls) ++ MarkedSymbol m :: map UnmarkedSymbol rs ++ [RightBlank false]
+      end*)
+    Notation sig__M := (FinType(EqType(sigTape sig))).
+    
+    Definition d__sig :sigTape sig := NilBlank.
+    Definition Rel : pRel sig__M bool 1 := ContainsEncoding.Rel d__sig (encode_tape (sig:=sig)).
+
+    (*MOVE*)
+    Definition isLeftBorder {sig : Type} (s : sigTape sig) : bool :=
+      match s with
+      | LeftBlank _ | NilBlank => true
+      | _ => false
+      end.
+
+    (*MOVE*)
+    Definition isRightBorder {sig : Type} (s : sigTape sig) : bool :=
+      match s with
+      | RightBlank _ | NilBlank => true
+      | _ => false
+      end.
+
+    Let M2 x :pTM sig__M bool 1 := if negb (Option.apply (@isMarked sig) false x)
+                         then Return Nop false
+                         else
+                           MoveToSymbol (fun x => isMarked x || isLeftBorder x || isRightBorder x) id;;
+                                        Relabel ReadChar (Option.apply isRightBorder false).
+
+    Let M1 (x : option (sigTape sig)): pTM sig__M bool 1:=
+           match x with
+             Some NilBlank => Return Nop true
+           | Some (LeftBlank b) =>
+             (if b then Nop
+              else Move R;; 
+                        MoveToSymbol (fun x => isMarked x || isLeftBorder x || isRightBorder x) id
+             );;
+              Switch ReadChar M2
+                  
+           | _ => Return Nop false
+           end.
+    
+    Definition M : pTM sig__M bool 1  :=
+      Switch
+        ReadChar M1.
+
+    (** Verification*)
+    
+    
+    Local Arguments Vector.to_list {A n} (!v).
+    
+    Local Arguments plus : simpl never.
+    Local Arguments mult : simpl never.
+
+
+    (*
+    Lemma Realises : M ⊨ Rel.
+    Proof.
+      eapply Realise_monotone.
+      { unfold M. TM_Correct.
+        all:unfold M1. all:TM_Correct.
+        all:unfold M2. all:cbn;TM_Correct.
+      }
+      { unfold Rel,ContainsEncoding.Rel. TMSimp. eauto. }
+      eapply TerminatesIn_monotone.
+      { unfold M. TM_Correct.
+        - apply Step_Realise.
+        - apply Step_Terminates. }
+      { revert q. apply StateWhileCoInduction; intros q; intros. destruct HT as (T&kn&outc&HLoop&HEncT&Hk). rewrite Loop_steps_eq in Hk. unfold Step_T, Step_Rel.
+        destruct (halt q) eqn:E; cbn in *.
+        - exists 0. split; auto. intros ymid tmid HStep. specialize HStep with (1 := HEncT) as (HStep&->). auto.
+        - destruct kn as [ | kn']; cbn in *.
+          + unfold haltConf in HLoop. cbn in HLoop. rewrite E in HLoop. congruence.
+          + unfold haltConf in HLoop. cbn in HLoop. rewrite E in HLoop.
+            destruct (trans (q, current_chars T)) as [q' acts] eqn:E2.
+            exists (Step_steps q T). repeat split. eauto.
+            intros ymid tmid HStep. specialize HStep with (1 := HEncT).
+            assert (step (mk_mconfig q T) = mk_mconfig q' (doAct_multi T acts)) as Hstep.
+            { unfold step. cbn. rewrite E2. reflexivity. }
+            rewrite Hstep in HStep. destruct HStep as (HStep&->).
+            exists (Loop_steps q' (doAct_multi T acts) kn'). repeat split; auto.
+            hnf. do 3 eexists. repeat split. 2: eauto. rewrite <- Hstep. eauto. eauto.
+      }
+    Qed.*)
+    
+    Definition Ter : tRel sig__M 1:=
+      fun tin k => 10 + sizeOfTape tin[@Fin0]*cnst 1 <= k.
+
+    Lemma Terminates : projT1 M ↓ Ter.
+    Proof.
+      eapply TerminatesIn_monotone.
+      { unfold M. TM_Correct.
+        all:unfold M1. all:TM_Correct.
+        all:unfold M2. all:cbn;TM_Correct.
+      }
+      { intros tin k Hk. evar (k0:nat). enough (k0=k) as Hk0. rewrite <- Hk0. unfold k0.
+        Tactic Notation "infArgs" int_or_var(n) := do n (try first [eexists | reflexivity]).
+        cbn. infArgs 5.  intros ? ? [-> ->].
+        (*TODO: unify cases *)
+    Abort.
+    
+  End checkEncodesTape.
+End CheckEncodesTape.
+
+(*
+Module CheckEncodesTapes.
+  Section checkEncodesTapes.
+    Import EncodeTapes StateWhile CaseList.
+    Context (sig:finType) (n:nat).
+
+    Eval cbv in encode_tapes [| niltape nat; midtape [3;2;1] 4 [5;6;7]; leftof 1 [2;3];rightof 3 [2;1] |].
+    
+    Definition M__Rel : pRel sig 1
+
+    Definition state := option (Fin.t n).
+    
+    
+    Definition Step : pTM sig (state + bool) 1 := _.
+    
+    Definition M := StateWhile Step__CheckEncodeTapes. 
+    End checkEncodeTapes.
+ *)
+
+Section multiToMono.
+  
+  Import EncodeTapes.
+  Context (sig F:finType) (n:nat) `{R__sig : registered sig}  (M : pTM sig F (S n)).
+
+  Eval cbn in (StepTM.ToSingleTape M).
+
+  
+
+End multiToMono.
 
 Lemma LMGenNP_to_TMGenNP_mTM (sig:finType) (n:nat) `{R__sig : registered sig}  (M : mTM sig (S n)):
   exists sig' `{R__sig' : registered sig'} (M' : mTM sig 1),
     restrictBy (HaltsOrDiverges_fixed_mTM M) (TMGenNP_fixed_mTM M)
                ⪯p unrestrictedP (TMGenNP_fixed_singleTapeTM M').
 Proof.
+  
 Abort.
